Escallon/LR_Parsing/Item_Pushdown_Automata.thy
@@ -1,0 +1,414 @@
+theory Item_Pushdown_Automata
+  imports 
+    Extended_Cfg
+    Pushdown_Automata.Pushdown_Automata
+begin
+
+ (* Better? *)
+(* locale ipda = Extended_Cfg G for G :: "('n::fresh0, 't) Cfg" +
+  fixes M :: "(('n, 't) item, 't, ('n, 't) item) pda"
+  assumes init_state:   "init_state M = [S' \<rightarrow> [] . [Nt S]]"
+      and init_symbol:  "init_symbol M = [S' \<rightarrow> [] . []]"
+      and final_states: "final_states M = {[S' \<rightarrow> [Nt S] . []]}"
+      and delta:        "delta M = (\<lambda>q a s. case q of [X \<rightarrow> \<beta> . Tm a' # \<gamma>] \<Rightarrow> 
+           if a' = a then let r = [X \<rightarrow> \<beta> @ [Tm a] . \<gamma>] in {(r, [s])} else {} | _ \<Rightarrow> {})"
+      and delta_eps:    "delta_eps M = (\<lambda>q s. case (q,s) of 
+      ([X \<rightarrow> \<beta> . Nt Y # \<gamma>], _) \<Rightarrow> {([Y \<rightarrow> [] . \<alpha>], [X \<rightarrow> \<beta> . Nt Y#\<gamma>]#[s]) |\<alpha>. (Y,\<alpha>) \<in> Prods G'} |
+      ([Y \<rightarrow> \<alpha> . []], [X \<rightarrow> \<beta> . Nt Y' # \<gamma>]) 
+        \<Rightarrow> if Y = Y' then {([X \<rightarrow> \<beta>@[Nt Y] . \<gamma>], [])} else {} | _ \<Rightarrow> {})" *)
+
+
+
+context Extended_Cfg
+begin
+
+definition IPDA :: "(('n, 't) item, 't, ('n, 't) item) pda" where
+  "IPDA \<equiv> let
+    P = Prods G';
+    \<delta> = (\<lambda>q a s. case q of [X \<rightarrow> \<beta> . Tm a' # \<gamma>] \<Rightarrow> 
+            if a' = a then let r = [X \<rightarrow> \<beta> @ [Tm a] . \<gamma>] in {(r, [s])} else {} | _ \<Rightarrow> {});
+    \<E> = (\<lambda>q s. case (q,s) of 
+      ([X \<rightarrow> \<beta> . Nt Y # \<gamma>], _) \<Rightarrow> {([Y \<rightarrow> [] . \<alpha>], [X \<rightarrow> \<beta> . Nt Y#\<gamma>]#[s]) |\<alpha>. (Y,\<alpha>) \<in> P} |
+      ([Y \<rightarrow> \<alpha> . []], [X \<rightarrow> \<beta> . Nt Y' # \<gamma>]) 
+        \<Rightarrow> if Y = Y' then {([X \<rightarrow> \<beta>@[Nt Y] . \<gamma>], [])} else {} | _ \<Rightarrow> {})         
+in
+  \<lparr>init_state = [S' \<rightarrow> [] . [Nt S]], init_symbol = [S' \<rightarrow> [] . []], 
+    final_states = {[S' \<rightarrow> [Nt S] . []]}, delta = \<delta>, delta_eps = \<E>\<rparr>"
+
+lemma init_state_IPDA [simp]:
+  "init_state IPDA = [S' \<rightarrow> [] . [Nt S]]"
+  unfolding IPDA_def by simp
+
+lemma init_symbol_IPDA [simp]:
+  "init_symbol IPDA = [S' \<rightarrow> [] . []]"
+  unfolding IPDA_def by simp
+
+lemma final_states_IPDA [simp]:
+  "final_states IPDA = {[S' \<rightarrow> [Nt S] . []]}"
+  unfolding IPDA_def by simp
+
+lemma delta_IPDA [simp]:
+  "delta IPDA = (\<lambda>q a s. case q of [X \<rightarrow> \<beta> . Tm a' # \<gamma>] \<Rightarrow> 
+            if a' = a then let r = [X \<rightarrow> \<beta> @ [Tm a] . \<gamma>] in {(r, [s])} else {} | _ \<Rightarrow> {})"
+  unfolding IPDA_def by auto
+
+lemma delta_eps_IPDA [simp]:
+  "delta_eps IPDA = (\<lambda>q s. case (q,s) of 
+      ([X \<rightarrow> \<beta> . Nt Y # \<gamma>], _) \<Rightarrow> {([Y \<rightarrow> [] . \<alpha>], [X \<rightarrow> \<beta> . Nt Y#\<gamma>]#[s]) |\<alpha>. (Y,\<alpha>) \<in> Prods G'} |
+      ([Y \<rightarrow> \<alpha> . []], [X \<rightarrow> \<beta> . Nt Y' # \<gamma>]) 
+        \<Rightarrow> if Y = Y' then {([X \<rightarrow> \<beta>@[Nt Y] . \<gamma>], [])} else {} | _ \<Rightarrow> {})"
+  unfolding IPDA_def by simp
+
+lemma delta_complete_empty [simp]:
+  "delta IPDA ([X \<rightarrow> \<alpha> . []]) a q = {}"
+  unfolding IPDA_def by simp
+
+lemma delta_Nt_empty [simp]:
+  "delta IPDA ([X \<rightarrow> \<alpha> . Nt A # \<gamma>]) a q = {}"
+  unfolding IPDA_def by auto
+
+lemma delta_Tm_neq_empty [simp]:
+  assumes "a \<noteq> b"
+  shows "delta IPDA ([X \<rightarrow> \<alpha> . Tm a # \<gamma>]) b q = {}"
+  using assms unfolding IPDA_def by simp
+
+lemma delta_nempty_impl_Tm_eq:
+  assumes "delta IPDA p a q \<noteq> {}"
+  obtains X \<beta> \<gamma> where "p = [X \<rightarrow> \<beta> . Tm a # \<gamma>]"
+proof -
+  obtain X \<beta> \<alpha> where p_def: "p = [X \<rightarrow> \<beta> . \<alpha>]" using item.exhaust by blast
+  then consider (Nil) "\<alpha> = []" | (Tm_eq) \<gamma> where "\<alpha> = Tm a # \<gamma>" | 
+   (Tm_neq) a' \<gamma> where "\<alpha> = Tm a' # \<gamma>" "a' \<noteq> a" | (Nt) A \<gamma> where "\<alpha> = Nt A # \<gamma>"
+    using list.exhaust sym.exhaust by metis
+  then show thesis using p_def assms that by cases auto
+qed
+
+lemma delta_eps_Tm_empty [simp]:
+   "delta_eps IPDA ([X \<rightarrow> \<alpha> . Tm a # \<gamma>]) q = {}"
+  unfolding IPDA_def by simp
+
+lemma delta_eps_Nt_neq_empty [simp]:
+  assumes "Y \<noteq> Y'"
+  shows "delta_eps IPDA ([Y \<rightarrow> \<alpha> . []]) ([X \<rightarrow> \<beta> . Nt Y' # \<gamma>]) = {}"
+  using assms unfolding IPDA_def by simp
+
+(* TODO: case nempty? *)
+lemma delta_eps_nempty_impl_expanding_or_reducing:
+  assumes "delta_eps IPDA "
+
+
+type_synonym ('q,'s) ipda_config = "'q list \<times> 's list"
+
+lemmas init_defs = init_state_def init_symbol_def
+
+abbreviation "final_state \<equiv> [S' \<rightarrow> [Nt S] . []]"
+
+lemma in_final_impl_final_state:
+  assumes "q \<in> final_states IPDA"
+  shows "q = final_state"
+  using assms unfolding IPDA_def S'_def S_def by simp
+
+lemma final_state_in_final[simp]:
+  "final_state \<in> final_states IPDA"
+  unfolding IPDA_def S'_def S_def by simp
+
+
+
+lemma delta_init_empty:
+  "delta IPDA (init_state IPDA) a (init_symbol IPDA) = {}"
+proof -
+  let ?\<delta> = "(\<lambda>q a s. case q of [X \<rightarrow> \<beta> . Tm a' # \<gamma>] \<Rightarrow> 
+            if a' = a then let r = [X \<rightarrow> \<beta> @ [Tm a] . \<gamma>] in {(r, [s])} else {} | _ \<Rightarrow> {})"
+  have delta: "?\<delta> = delta IPDA"  unfolding IPDA_def by simp
+  from init_state_def have "?\<delta> (init_state IPDA) a (init_symbol IPDA) = {}" 
+    by auto
+  with ext delta show ?thesis  by (metis (lifting))
+qed
+
+inductive step :: "(('n,'t) item,'t) ipda_config \<Rightarrow> (('n,'t) item,'t) ipda_config \<Rightarrow> bool" (infix \<open>\<turnstile>P\<close> 70) where
+delta[intro]: "\<lbrakk>\<alpha> = [p0, p1]; \<alpha>' = q#qs; (q,qs) \<in> delta IPDA p0 a p1\<rbrakk> 
+                \<Longrightarrow> (\<alpha>@\<beta>,a#w) \<turnstile>P (\<alpha>'@\<beta>,w)" |
+eps[intro]: "\<lbrakk>\<alpha> = [p0, p1]; \<alpha>' = q#qs; (q,qs) \<in> delta_eps IPDA p0 p1\<rbrakk> 
+                \<Longrightarrow> (\<alpha>@\<beta>, w) \<turnstile>P (\<alpha>'@\<beta>, w)"
+
+inductive_cases step_deltaE[elim]: "(s, x#w) \<turnstile>P (s', w)"
+inductive_cases step_epsE[elim]: "(s, w) \<turnstile>P (s', w)"
+
+lemma step_equal_or_Cons:
+  assumes "(p,u) \<turnstile>P (q,v)"
+  shows "u = v \<or> (\<exists>a. u = a#v)"
+  using assms by cases auto
+
+lemma step_len_dec:
+  assumes "(p,u) \<turnstile>P (q,v)"
+  shows "length u \<ge> length v" 
+  using step_equal_or_Cons[OF assms] by fastforce
+
+
+
+lemma shifting[simp]:
+  "([A \<rightarrow> \<alpha> . Tm a # \<beta>]#\<rho>#\<rho>s, a#u) \<turnstile>P ([A \<rightarrow> \<alpha>@[Tm a] . \<beta>]#\<rho>#\<rho>s, u)"
+proof -
+  have "([A \<rightarrow> \<alpha>@[Tm a] . \<beta>], [\<rho>]) \<in> delta IPDA ([A \<rightarrow> \<alpha> . Tm a # \<beta>]) a \<rho>"
+    using IPDA_def by simp
+  then show ?thesis using delta 
+    by (metis Cons_eq_appendI append.left_neutral)
+qed
+
+
+lemma reducing[simp]:
+  "([Y \<rightarrow> \<alpha> . []]#[X \<rightarrow> \<beta> . Nt Y#\<gamma>]#\<rho>, w) \<turnstile>P ([X \<rightarrow> \<beta> @ [Nt Y] . \<gamma>]#\<rho>, w)"
+proof -
+  have "([X \<rightarrow> \<beta> @ [Nt Y] . \<gamma>], []) \<in> delta_eps IPDA ([Y \<rightarrow> \<alpha> . []]) ([X \<rightarrow> \<beta> . Nt Y#\<gamma>])"
+    unfolding IPDA_def by simp
+  thus ?thesis using eps by (metis Cons_eq_appendI append.left_neutral)
+qed
+
+lemma expanding_in_delta_eps:
+  assumes "(Y, \<alpha>) \<in> Prods G'"
+  shows "([Y \<rightarrow> [] . \<alpha>], [[X \<rightarrow> \<beta> . Nt Y#\<gamma>], i]) \<in> delta_eps IPDA ([X \<rightarrow> \<beta> . Nt Y#\<gamma>]) i"
+  using assms unfolding G'_def S'_def S_def IPDA_def by auto
+
+lemma expanding[simp]:
+  assumes "(Y, \<alpha>) \<in> Prods G'"
+  shows "([X \<rightarrow> \<beta> . Nt Y#\<gamma>]#i#\<rho>, w) \<turnstile>P ([Y \<rightarrow> [] . \<alpha>]#[X \<rightarrow> \<beta> . Nt Y#\<gamma>]#i#\<rho>, w)"
+  using expanding_in_delta_eps[OF assms] eps 
+  by (metis eq_Nil_appendI Cons_eq_appendI)
+
+lemma in_delta_impl_shifting:
+  assumes "(q, qs) \<in> delta IPDA p0 a p1"
+  obtains X \<beta> \<gamma> where "p0 = [X \<rightarrow> \<beta> . Tm a # \<gamma>]"
+    "(q,qs) = ([X \<rightarrow> \<beta> @ [Tm a] . \<gamma>], [p1])"
+proof -
+  from assms have nempty: "delta IPDA p0 a p1 \<noteq> {}" by auto
+  let ?\<delta> = "(\<lambda>q a s. case q of [X \<rightarrow> \<beta> . Tm a' # \<gamma>] \<Rightarrow> 
+            if a' = a then let r = [X \<rightarrow> \<beta> @ [Tm a] . \<gamma>] in {(r, [s])} else {} | _ \<Rightarrow> {})"
+  have \<delta>_def: "?\<delta> = delta IPDA" unfolding IPDA_def by simp
+  from delta_nempty_impl_Tm_eq[OF nempty] 
+    obtain X \<beta> \<gamma> where p0_def: "p0 = [X \<rightarrow> \<beta> . Tm a # \<gamma>]" 
+    by blast
+  hence "?\<delta> p0 a p1 = {([X \<rightarrow> \<beta> @ [Tm a] . \<gamma>], [p1])}" by simp
+  with assms show thesis using \<delta>_def that p0_def 
+    by (metis (lifting) singletonD)
+qed
+
+lemma eps_cases[consumes 1, case_names reducing expanding]:
+  assumes "(q0,q1) \<in> delta_eps IPDA p0 p1"
+  obtains Y \<alpha> X \<beta> \<gamma> where
+    "p0 = [Y \<rightarrow> \<alpha> . []]" "p1 = [X \<rightarrow> \<beta> . Nt Y # \<gamma>]" "q0 = [X \<rightarrow> \<beta> @ [Nt Y] . \<gamma>]" "q1 = []" |
+    X \<beta> Y \<gamma> \<alpha> where
+    "p0 = [X \<rightarrow> \<beta> . Nt Y # \<gamma>]" "(Y, \<alpha>) \<in> Prods G'" "q0 = [Y \<rightarrow> [] . \<alpha>]" "q1 = [p0]" 
+proof -
+  let ?\<delta> = "(\<lambda>q s. case (q,s) of 
+      ([X \<rightarrow> \<beta> . Nt Y # \<gamma>], _) \<Rightarrow> {([Y \<rightarrow> [] . \<alpha>], [X \<rightarrow> \<beta> . Nt Y#\<gamma>]#[s]) |\<alpha>. (Y,\<alpha>) \<in> Prods G'} |
+      ([Y \<rightarrow> \<alpha> . []], [X \<rightarrow> \<beta> . Nt Y' # \<gamma>]) 
+        \<Rightarrow> if Y = Y' then {([X \<rightarrow> \<beta>@[Nt Y] . \<gamma>], [])} else {} | _ \<Rightarrow> {})"
+  have "delta_eps IPDA = ?\<delta>"
+    using delta_eps_IPDA S_def S'_def G'_def by fastforce
+  with assms
+  show thesis sorry
+qed
+
+lemma step_cases[consumes 1, case_names shifting reducing expanding]:
+  assumes "c0 \<turnstile>P c1"
+obtains A \<alpha> a \<beta> i \<rho> u where 
+    "c0 = ([A \<rightarrow> \<alpha> . Tm a # \<beta>]#i#\<rho>, a#u)" "c1 = ([A \<rightarrow> \<alpha>@[Tm a] . \<beta>]#i#\<rho>, u)" |
+    Y \<alpha> X \<beta> \<gamma> \<rho> w where
+      "c0 = ([Y \<rightarrow> \<alpha> . []]#[X \<rightarrow> \<beta> . Nt Y#\<gamma>]#\<rho>, w)"  "c1 = ([X \<rightarrow> \<beta> @ [Nt Y] . \<gamma>]#\<rho>, w)" |
+    Y \<alpha> X \<beta> \<gamma> i \<rho> w where 
+    "c0 = ([X \<rightarrow> \<beta> . Nt Y#\<gamma>]#i#\<rho>, w)"  "c1 = ([Y \<rightarrow> [] . \<alpha>]#[X \<rightarrow> \<beta> . Nt Y#\<gamma>]#i#\<rho>, w)"
+      "(Y, \<alpha>) \<in> Prods G'"
+  using assms proof cases
+  case (delta \<alpha> p0 p1 \<alpha>' q qs a \<beta> w)
+  thm IPDA_def
+  from in_delta_impl_shifting[OF delta(5)] obtain X \<beta>' \<gamma> where "p0 = [X \<rightarrow> \<beta>' . Tm a # \<gamma>]" 
+    "(q,qs) = ([X \<rightarrow> \<beta>' @ [Tm a] . \<gamma>], [p1])" by blast
+  then show ?thesis using that delta by simp 
+next
+  case (eps \<alpha> p0 p1 \<alpha>' q qs \<beta> w)
+  from eps(5) show ?thesis 
+    by (cases rule: eps_cases) 
+      (use eps that in simp, 
+        use expanding_in_delta_eps eps_cases in blast)
+qed
+
+lemma step_impl_in_It:
+  assumes "i \<in> It G'"
+    "(i#is, u) \<turnstile>P (j#js, v)"
+  shows "j \<in> It G'"
+  using [[simp_trace]]
+  using assms(2) apply (cases rule: step_cases)
+  using assms apply (simp_all add: items_of_Prods_def)[2]
+  using assms sorry 
+
+
+lemma 
+  assumes "([A \<rightarrow> \<alpha> . \<beta>]#\<rho>, u) \<turnstile>P c"
+  shows "Prods G' \<turnstile> [Nt A] \<Rightarrow> \<alpha>@\<beta>"
+  using assms apply cases
+  sorry
+
+
+abbreviation steps (infix \<open>\<turnstile>P*\<close> 70) where
+  "steps \<equiv> (step \<^sup>*\<^sup>*)"
+
+abbreviation stepn ( \<open>_ \<turnstile>P'(_') _\<close> 70) where
+  "stepn c0 n c1 \<equiv> (step ^^ n) c0 c1"
+
+lemma steps_len_dec:
+  "(p,u) \<turnstile>P* (q,v) \<Longrightarrow> length u \<ge> length v" 
+  by ((induction "(p,u)" "(q,v)" arbitrary: q v rule: rtranclp.induct),
+  (use step_len_dec surj_pair le_trans in fastforce)+)
+
+lemma syms_complete:
+  "([A \<rightarrow> \<alpha> . map Tm u @ \<beta>]#i#is, u@v) \<turnstile>P* ([A \<rightarrow> \<alpha> @ map Tm u . \<beta>]#i#is, v)"
+proof (induction u arbitrary: \<alpha>)
+  case (Cons a u)
+  have "([A \<rightarrow> \<alpha> . map Tm (a # u) @ \<beta>] # i # is, (a # u) @ v) 
+        \<turnstile>P ([A \<rightarrow> \<alpha> @ [Tm a] . map Tm u @ \<beta>] # i # is, u @ v)"
+    by simp
+  also note Cons[of "\<alpha>@[Tm a]"] 
+  finally show ?case by auto
+qed simp
+
+lemma reachable_impl_in_It:
+  assumes "(init_state IPDA#\<rho>0, u) \<turnstile>P* (\<rho>1, v)"
+  shows "\<forall>i \<in> set \<rho>1. i \<in> It G'"
+  sorry
+
+
+lemma steps_substring:
+  assumes "(\<rho>0, w) \<turnstile>P* (\<rho>2, v)"
+  obtains u where "w = u@v"
+  sorry
+
+lemma list_app_last_is_next_hd:
+  assumes "w = u@v@y"
+    "w = xs@a#y"
+    "v \<noteq> []"
+  shows "last v = a"
+  using assms 
+  by (metis append.assoc append_Cons append_Nil append_same_eq last_append last_snoc)
+
+lemma reachable_impl_reachable_substring:
+  assumes "(\<rho>0, u) \<turnstile>P* (\<rho>2, y)"
+    "u = v@w@y"
+  obtains \<rho>1 where "(\<rho>0, u) \<turnstile>P* (\<rho>1, w@y)"
+proof -
+  from assms(1) obtain n where "(\<rho>0, u) \<turnstile>P(n) (\<rho>2, y)"
+    by (metis rtranclp_imp_relpowp)
+  with assms(2) obtain \<rho>1 where "(\<rho>0, u) \<turnstile>P* (\<rho>1, w@y)"
+  proof (induction n arbitrary: \<rho>2 v w y thesis rule: less_induct)
+    case (less n)
+    show ?case 
+    proof (cases n)
+      case (Suc m)
+      with less(4) obtain \<rho>1 z where msteps: "(\<rho>0, u) \<turnstile>P(m) (\<rho>1, z)" "(\<rho>1, z) \<turnstile>P (\<rho>2, y)" by auto
+      from msteps(2) consider "z = y" | a where "z = a#y" using step.cases by blast
+      then show ?thesis
+      proof cases
+        case 1
+        with less(1,3) msteps(1) Suc obtain \<rho>' where "(\<rho>0, u) \<turnstile>P* (\<rho>', w @ y)" by blast
+        then show ?thesis using less(2) by blast
+      next
+        case 2
+        with msteps steps_substring obtain as where as: "u = as@a#y" 
+          by (meson rtranclp_power)
+        show ?thesis 
+        proof (cases w)
+          case (Cons b bs)
+          then obtain cs where cs_def: "w = cs @ [a]" 
+            using as list_app_last_is_next_hd[OF less(3)] 
+            by (metis list.distinct(1) snoc_eq_iff_butlast)
+          hence "u = v @ cs @ z" using less 2 by simp
+          from less(1)[OF _ _ this msteps(1)] obtain \<rho>' where "(\<rho>0, u) \<turnstile>P* (\<rho>', cs @ z)"
+            using Suc by blast
+          then show ?thesis using cs_def 2 less(2) by simp
+        qed (use less rtranclp_power append_Nil in metis)
+      qed
+    qed (use less that in auto)
+  qed
+  then show thesis using that by blast
+qed
+
+
+lemma syms_tl_impl_substring:
+  assumes "([A \<rightarrow> \<alpha> . \<beta> @ map Tm u]#\<rho>, v) \<turnstile>P* ([A \<rightarrow> \<alpha>@\<beta>@map Tm u . []]#\<rho>', w)"
+  obtains v' where "v = v'@u"
+  sorry
+
+lemma reaches_final_impl_reaches_complete:
+  assumes "([A \<rightarrow> \<alpha> . \<beta>]#\<rho>, v) \<turnstile>P* ([[S' \<rightarrow> [Nt S] . []], init_symbol IPDA], [])"
+  obtains w where "([A \<rightarrow> \<alpha> . \<beta>]#\<rho>, v) \<turnstile>P* ([A \<rightarrow> \<alpha>@\<beta> . []]#\<rho>', w)"
+  sorry
+
+corollary reaches_final_impl_substring:
+  assumes "([A \<rightarrow> \<alpha> . \<beta> @ map Tm u]#\<rho>, v) \<turnstile>P* ([[S' \<rightarrow> [Nt S] . []], init_symbol IPDA], [])"
+  obtains v' where "v = v'@u"
+  using reaches_final_impl_reaches_complete[OF assms, THEN syms_tl_impl_substring]
+  by metis
+
+lemma reaches_final_impl_interm_reaches_final:
+  assumes "c0 \<turnstile>P* ([[S' \<rightarrow> [Nt S] . []], init_symbol IPDA], [])"
+    "c0 \<turnstile>P* c1"
+  shows "c1 \<turnstile>P* ([[S' \<rightarrow> [Nt S] . []], init_symbol IPDA], [])"
+  sorry
+
+
+
+definition ipda_Lang :: "'t list set" where
+  "ipda_Lang \<equiv> {w. ([init_state IPDA, init_symbol IPDA], w)
+             \<turnstile>P* ([[S' \<rightarrow> [Nt S] . []], init_symbol IPDA], [])}"
+
+
+lemma hist_singleton_init [simp]:
+  "hist ([[A \<rightarrow> \<alpha> . \<beta>], init_symbol IPDA]) = \<alpha>"
+  unfolding IPDA_def using hist_singleton by auto
+
+lemma hist_init [simp]:
+  "hist (\<rho>@[init_symbol IPDA]) = hist \<rho>"
+  using IPDA_def by (induction \<rho>) auto
+
+lemma invariant: 
+  assumes "([init_state IPDA, init_symbol IPDA], u@v) \<turnstile>P* (\<rho>, v)"
+  shows "Prods G \<turnstile> hist \<rho> \<Rightarrow>* map Tm u"
+  sorry
+
+corollary ipda_Lang_subst_Lang_G:
+  "ipda_Lang \<subseteq> LangS G"
+  unfolding ipda_Lang_def Context_Free_Grammar.Lang_def S_def 
+  by (standard, metis invariant append.right_neutral hist_singleton_init mem_Collect_eq)
+
+lemma derives_impl_completes:
+  assumes "Prods G \<turnstile> [Nt A] \<Rightarrow> \<alpha>"
+    "Prods G \<turnstile> \<alpha> \<Rightarrow>* map Tm w"
+  shows "([A \<rightarrow> [] . \<alpha>]#\<rho>, w@v) \<turnstile>P* ([A \<rightarrow> \<alpha> . []]#\<rho>, v)"
+  sorry
+
+
+lemma ipda_Lang_eq_Lang_G:
+  "ipda_Lang = LangS G"
+  sorry
+
+
+lemma first_step_is_eps:
+  assumes "([init_state IPDA, init_symbol IPDA], u) \<turnstile>P* (qs, v)"
+    "([init_state IPDA, init_symbol IPDA], u) \<noteq> (qs, v)"
+  obtains \<alpha> where 
+    "([init_state IPDA, init_symbol IPDA], u) \<turnstile>P ([[S \<rightarrow> [] . \<alpha>], init_state IPDA, init_symbol IPDA], u)"
+    "([[S \<rightarrow> [] . \<alpha>], init_state IPDA, init_symbol IPDA], u) \<turnstile>P* (qs, v)"
+proof -
+  from assms obtain ps u' where step: "([init_state IPDA, init_symbol IPDA], u) \<turnstile>P (ps, u')"
+    and steps: "(ps, u') \<turnstile>P* (qs, v)"
+    by (metis converse_rtranclpE2)
+  moreover have "u = u'" 
+    by (rule ccontr, use step delta_init_empty step_equal_or_Cons in fastforce)
+  moreover with step obtain r rs where 
+    "ps = r#rs" "(r, rs) \<in> delta_eps IPDA (init_state IPDA) (init_symbol IPDA)"
+    using step_epsE by fastforce 
+  ultimately show thesis using that by auto
+qed
+
+end
+
+end
